Lean4Lean/Theory/Typing/Strong.lean
@@ -13,18 +13,23 @@ variable (env : VEnv) (uvars : Nat)
 
 inductive IsDefEqStrong : List VExpr → VExpr → VExpr → VExpr → Prop where
   | bvar : Lookup Γ i A → u.WF uvars → Γ ⊢ A : .sort u → Γ ⊢ .bvar i : A
-  | const :
-    env.constants c = some (some ci) →
-    (∀ l ∈ ls, l.WF uvars) →
-    ls.length = ci.uvars →
-    u.WF uvars →
-    [] ⊢ ci.type.instL ls : .sort u →
-    Γ ⊢ .const c ls : ci.type.instL ls
   | symm : Γ ⊢ e ≡ e' : A → Γ ⊢ e' ≡ e : A
   | trans : Γ ⊢ e₁ ≡ e₂ : A → Γ ⊢ e₂ ≡ e₃ : A → Γ ⊢ e₁ ≡ e₃ : A
   | sortDF :
     l.WF uvars → l'.WF uvars → l ≈ l' →
     Γ ⊢ .sort l ≡ .sort l' : .sort (.succ l)
+  | constDF :
+    env.constants c = some (some ci) →
+    (∀ l ∈ ls, l.WF uvars) →
+    (∀ l ∈ ls', l.WF uvars) →
+    ls.length = ci.uvars →
+    List.Forall₂ (· ≈ ·) ls ls' →
+    u.WF uvars →
+    [] ⊢ ci.type.instL ls : .sort u →
+    [] ⊢ ci.type.instL ls' : .sort u →
+    Γ ⊢ ci.type.instL ls : .sort u →
+    Γ ⊢ ci.type.instL ls' : .sort u →
+    Γ ⊢ .const c ls ≡ .const c ls' : ci.type.instL ls
   | appDF :
     u.WF uvars → v.WF uvars →
     Γ ⊢ A : .sort u →
@@ -88,12 +93,12 @@ theorem IsDefEqStrong.weakN (W : Ctx.LiftN n k Γ Γ') (H : env.IsDefEqStrong U 
     env.IsDefEqStrong U Γ' (e1.liftN n k) (e2.liftN n k) (A.liftN n k) := by
   induction H generalizing k Γ' with
   | bvar h1 h2 h3 => refine .bvar (h1.weakN W) h2 (h3.weakN W)
-  | const h1 h2 h3 h4 h5 =>
-    rw [(henv.closedC h1).instL.liftN_eq (Nat.zero_le _)]
-    exact .const h1 h2 h3 h4 h5
   | symm _ ih => exact .symm (ih W)
   | trans _ _ ih1 ih2 => exact .trans (ih1 W) (ih2 W)
   | sortDF h1 h2 h3 => exact .sortDF h1 h2 h3
+  | constDF h1 h2 h3 h4 h5 h6 h7 h8 _ _ _ _ ih3 ih4 =>
+    simp [(henv.closedC h1).instL.liftN_eq (Nat.zero_le _)] at ih3 ih4 ⊢
+    exact .constDF h1 h2 h3 h4 h5 h6 h7 h8 (ih3 W) (ih4 W)
   | appDF h1 h2 _ _ _ _ _ ih1 ih2 ih3 ih4 ih5 =>
     refine liftN_inst_hi .. ▸ .appDF h1 h2 (ih1 W) (ih2 W.succ) (ih3 W) (ih4 W) ?_
     exact liftN_inst_hi .. ▸ liftN_inst_hi .. ▸ ih5 W
@@ -117,20 +122,19 @@ theorem IsDefEqStrong.weakN (W : Ctx.LiftN n k Γ Γ') (H : env.IsDefEqStrong U 
   | proofIrrel _ _ _ ih1 ih2 ih3 => exact .proofIrrel (ih1 W) (ih2 W) (ih3 W)
   | extra h1 h2 h3 h4 h5 h6 h7 _ _ _ _ _ ih4 ih5 =>
     have ⟨⟨hA1, _⟩, hA2, hA3⟩ := henv.closed.2 h1
-    specialize ih4 W; specialize ih5 W
     simp [
       hA1.instL.liftN_eq (Nat.zero_le _),
       hA2.instL.liftN_eq (Nat.zero_le _),
       hA3.instL.liftN_eq (Nat.zero_le _)] at ih4 ih5 ⊢
-    exact IsDefEqStrong.extra h1 h2 h3 h4 h5 h6 h7 ih4 ih5
+    exact IsDefEqStrong.extra h1 h2 h3 h4 h5 h6 h7 (ih4 W) (ih5 W)
 
 theorem IsDefEqStrong.defeq (H : IsDefEqStrong env U Γ e1 e2 A) : env.IsDefEq U Γ e1 e2 A := by
   induction H with
   | bvar h => exact .bvar h
-  | const h1 h2 h3 => exact .const h1 h2 h3
   | symm _ ih => exact .symm ih
   | trans _ _ ih1 ih2 => exact .trans ih1 ih2
   | sortDF h1 h2 h3 => exact .sortDF h1 h2 h3
+  | constDF h1 h2 h3 h4 h5 => exact .constDF h1 h2 h3 h4 h5
   | appDF _ _ _ _ _ _ _ _ _ ih1 ih2 => exact .appDF ih1 ih2
   | lamDF _ _ _ _ _ _ _ ih1 _ _ ih2 => exact .lamDF ih1 ih2
   | forallEDF _ _ _ _ _ ih1 ih2 => exact .forallEDF ih1 ih2
@@ -145,10 +149,11 @@ theorem IsDefEqStrong.mono
     (H : env.IsDefEqStrong U Γ e1 e2 A) : env'.IsDefEqStrong U Γ e1 e2 A := by
   induction H with
   | bvar h1 h2 _ ih => exact .bvar h1 h2 ih
-  | const h1 h2 h3 h4 _ ih => exact .const (henv.1 _ _ h1) h2 h3 h4 ih
-  | sortDF h1 h2 h3 => exact .sortDF h1 h2 h3
   | symm _ ih => exact .symm ih
   | trans _ _ ih1 ih2 => exact .trans ih1 ih2
+  | sortDF h1 h2 h3 => exact .sortDF h1 h2 h3
+  | constDF h1 h2 h3 h4 h5 h6 _ _ _ _ ih1 ih2 ih3 ih4 =>
+    exact .constDF (henv.1 _ _ h1) h2 h3 h4 h5 h6 ih1 ih2 ih3 ih4
   | appDF h1 h2 _ _ _ _ _ ih1 ih2 ih3 ih4 ih5 => exact .appDF h1 h2 ih1 ih2 ih3 ih4 ih5
   | lamDF h1 h2  _ _ _ _ _ ih1 ih2 ih3 ih4 ih5 => exact .lamDF h1 h2 ih1 ih2 ih3 ih4 ih5
   | forallEDF h1 h2 _ _ _ ih1 ih2 ih3 => exact .forallEDF h1 h2 ih1 ih2 ih3
@@ -172,9 +177,11 @@ theorem IsDefEqStrong.instL (H : env.IsDefEqStrong U Γ e1 e2 A) :
   induction H with
   | bvar h _ _ ih =>
     exact .bvar h.instL (.inst hls) ih
-  | const h1 h2 h3 h4 h5 ih =>
-    simp [VExpr.instL, VExpr.instL_instL] at ih ⊢
-    exact .const h1 (by simp [h2, VLevel.WF.inst hls]) (by simp [h3]) (.inst hls) ih
+  | constDF h1 h2 h3 h4 h5 _ _ _ _ _ ih1 ih2 ih3 ih4 =>
+    simp [VExpr.instL, VExpr.instL_instL] at ih1 ih2 ih3 ih4 ⊢
+    exact .constDF h1
+      (by simp [h2, VLevel.WF.inst hls]) (by simp [h3, VLevel.WF.inst hls]) (by simp [h4])
+      (by simpa using h5.imp fun _ _ => VLevel.inst_congr_l) (.inst hls) ih1 ih2 ih3 ih4
   | symm _ ih => exact .symm ih
   | trans _ _ ih1 ih2 => exact .trans ih1 ih2
   | sortDF _ _ h3 =>
@@ -232,12 +239,12 @@ theorem IsDefEqStrong.instN (W : Ctx.InstN Γ₀ e₀ A₀ k Γ₁ Γ) (H : env.
         let ⟨u, hty⟩ := hΓ.lookup henv .zero
         exact .bvar .zero (hty.defeq.sort_r henv hΓ.defeq) hty
       | succ h => exact (ih h hΓ.1).weakN henv .one
-  | const h1 h2 h3 h4 h5 =>
-    rw [(henv.closedC h1).instL.instN_eq (Nat.zero_le _)]
-    exact .const h1 h2 h3 h4 h5
   | symm _ ih => exact .symm (ih W hΓ)
   | trans _ _ ih1 ih2 => exact .trans (ih1 W hΓ) (ih2 W hΓ)
   | sortDF h1 h2 h3 => exact .sortDF h1 h2 h3
+  | constDF h1 h2 h3 h4 h5 h6 h7 h8 _ _ _ _ ih3 ih4 =>
+    simp [(henv.closedC h1).instL.instN_eq (Nat.zero_le _)] at ih3 ih4 ⊢
+    exact .constDF h1 h2 h3 h4 h5 h6 h7 h8 (ih3 W hΓ) (ih4 W hΓ)
   | appDF h1 h2 _ _ _ _ _ ih1 ih2 ih3 ih4 ih5 =>
     exact inst0_inst_hi .. ▸ .appDF h1 h2
       (ih1 W hΓ) (ih2 W.succ ⟨hΓ, _, ih1 W hΓ⟩)
@@ -275,12 +282,11 @@ theorem IsDefEqStrong.instN (W : Ctx.InstN Γ₀ e₀ A₀ k Γ₁ Γ) (H : env.
   | proofIrrel _ _ _ ih1 ih2 ih3 => exact .proofIrrel (ih1 W hΓ) (ih2 W hΓ) (ih3 W hΓ)
   | extra h1 h2 h3 h4 h5 h6 h7 _ _ _ _ _ ih4 ih5 =>
     have ⟨⟨hA1, _⟩, hA2, hA3⟩ := henv.closed.2 h1
-    specialize ih4 W hΓ; specialize ih5 W hΓ
     simp [
       hA1.instL.instN_eq (Nat.zero_le _),
       hA2.instL.instN_eq (Nat.zero_le _),
       hA3.instL.instN_eq (Nat.zero_le _)] at ih4 ih5 ⊢
-    exact .extra h1 h2 h3 h4 h5 h6 h7 ih4 ih5
+    exact .extra h1 h2 h3 h4 h5 h6 h7 (ih4 W hΓ) (ih5 W hΓ)
 
 theorem IsDefEqStrong.defeqDF_l (henv : Ordered env) (hΓ : CtxStrong env U Γ)
     (h1 : env.IsDefEqStrong U Γ A A' (.sort u))
@@ -353,16 +359,12 @@ theorem IsDefEqStrong.isType' (hΓ : CtxStrong env U Γ) (H : env.IsDefEqStrong 
     ∃ u, env.IsDefEqStrong U Γ A A (.sort u) := by
   induction H with
   | bvar h => exact hΓ.lookup henv h
-  | const h1 h2 =>
-    let ⟨_, h⟩ := envIH.1 h1
-    exact ⟨_, (h.1.instL h2).weak0 henv⟩
-  | proofIrrel h1 => exact ⟨_, h1⟩
-  | extra h1 h2 =>
-    have ⟨_, h⟩ := (envIH.2 h1).2.2.1
-    exact ⟨_, (h.instL h2).weak0 henv⟩
-  | sortDF h1 => exact ⟨_, .sortDF h1 h1 rfl⟩
   | symm _ ih => exact ih hΓ
   | trans _ _ ih1 => exact ih1 hΓ
+  | sortDF h1 => exact ⟨_, .sortDF h1 h1 rfl⟩
+  | constDF h1 h2 =>
+    let ⟨_, h⟩ := envIH.1 h1
+    exact ⟨_, (h.1.instL h2).weak0 henv⟩
   | appDF _ _ _ _ _ h4 _ _ _ ih3 =>
     let ⟨_, ih3⟩ := ih3 hΓ
     have ⟨_, _, ih3⟩ := ih3.forallE_inv' henv envIH hΓ (.inl rfl)
@@ -372,6 +374,10 @@ theorem IsDefEqStrong.isType' (hΓ : CtxStrong env U Γ) (H : env.IsDefEqStrong 
   | defeqDF _ h2 => exact ⟨_, h2.hasType.2⟩
   | beta _ _ _ h4 _ h6 => exact ⟨_, h6.hasType.1.instN henv hΓ .zero h4 hΓ⟩
   | eta _ _ _ _ _ _ _ _ _ _ ih => exact ih hΓ
+  | proofIrrel h1 => exact ⟨_, h1⟩
+  | extra h1 h2 =>
+    have ⟨_, h⟩ := (envIH.2 h1).2.2.1
+    exact ⟨_, (h.instL h2).weak0 henv⟩
 
 theorem IsDefEqStrong.instDF
     (henv : Ordered env) (hΓ : CtxStrong env U Γ) (hu : u.WF U) (hv : v.WF U)
@@ -407,12 +413,15 @@ theorem IsDefEq.strong' (hΓ : CtxStrong env U Γ)
   | bvar h =>
     let ⟨u, hA⟩ := hΓ.lookup henv h
     exact .bvar h (hA.defeq.sort_r henv (hctx hΓ)) hA
-  | @const _ _ ls' _ h1 h2 h3 =>
-    let ⟨u, h4⟩ := envIH.1 h1
-    exact .const h1 h2 h3 (.inst h2) (h4.1.instL h2)
   | symm _ ih => exact (ih hΓ).symm
   | trans _ _ ih1 ih2 => exact (ih1 hΓ).trans (ih2 hΓ)
   | sortDF h1 h2 h3 => exact .sortDF h1 h2 h3
+  | @constDF _ _ ls₁ ls₂ _ h1 h2 h3 h4 h5 =>
+    let ⟨u, h6⟩ := envIH.1 h1
+    have H1 := h6.1.instL h2
+    have H2 := IsDefEqStrong.defeqDF (u := .succ _) (.inst h2)
+      (.symm <| .sortDF (.inst h2) (.inst h3) (VLevel.inst_congr rfl h5)) <| h6.1.instL h3
+    exact .constDF h1 h2 h3 h4 h5 (.inst h2) H1 H2 (H1.weak0 henv) (H2.weak0 henv)
   | appDF _ _ ih1 ih2 =>
     let ⟨_, h3⟩ := (ih1 hΓ).isType' henv envIH hΓ
     let ⟨⟨u, hA⟩, ⟨v, hB⟩⟩ := h3.forallE_inv' henv envIH hΓ (.inl rfl)
@@ -475,3 +484,92 @@ theorem CtxStrong.strong (henv : Ordered env) (hΓ : OnCtx Γ (env.IsType U)) : 
 theorem IsDefEq.strong (henv : Ordered env) (hΓ : OnCtx Γ (env.IsType U))
     (H : env.IsDefEq U Γ e1 e2 A) : env.IsDefEqStrong U Γ e1 e2 A :=
   H.strong' henv henv.strong (.strong henv hΓ)
+
+variable (henv : Ordered env) (hΓ : OnCtx Γ (env.IsType U)) in
+theorem IsDefEq.app_inv'
+    (H : env.IsDefEq U Γ e1 e2 V) (eq : e1 = .app f a ∨ e2 = .app f a) :
+    ∃ A B, env.HasType U Γ f (.forallE A B) ∧ env.HasType U Γ a A := by
+  have H' := H.strong henv hΓ; clear H hΓ
+  induction H' with
+  | symm _ ih => exact ih eq.symm
+  | trans _ _ ih1 ih2
+  | proofIrrel _ _ _ _ ih1 ih2
+  | extra _ _ _ _ _ _ _ _ _ _ _ _ ih1 ih2 =>
+    obtain eq | eq := eq <;> [exact ih1 (.inl eq); exact ih2 (.inr eq)]
+  | appDF _ _ _ _ h1 h2 =>
+    obtain ⟨⟨⟩⟩ | ⟨⟨⟩⟩ := eq
+    · exact ⟨_, _, h1.defeq.hasType.1, h2.defeq.hasType.1⟩
+    · exact ⟨_, _, h1.defeq.hasType.2, h2.defeq.hasType.2⟩
+  | defeqDF _ _ _ _ ih2 => exact ih2 eq
+  | beta _ _ hA _ he he' _ _ _ _ _ _ _ ihee =>
+    obtain ⟨⟨⟩⟩ | eq := eq
+    · exact ⟨_, _, .lam hA.defeq he.defeq, he'.defeq⟩
+    · exact ihee (.inl eq)
+  | eta _ _ _ _ _ _ _ _ _ _ ih =>
+    obtain ⟨⟨⟩⟩ | eq := eq
+    exact ih (.inl eq)
+  | _ => match eq with.
+
+variable (henv : Ordered env) (hΓ : OnCtx Γ (env.IsType U)) in
+theorem HasType.app_inv (H : env.HasType U Γ (.app f a) V) :
+    ∃ A B, env.HasType U Γ f (.forallE A B) ∧ env.HasType U Γ a A :=
+  H.app_inv' henv hΓ (.inl rfl)
+
+variable (henv : Ordered env) (hΓ : OnCtx Γ (env.IsType U)) in
+theorem IsDefEq.lam_inv'
+    (H : env.IsDefEq U Γ e1 e2 V) (eq : e1 = .lam A body ∨ e2 = .lam A body) :
+    env.IsType U Γ A ∧ ∃ B, env.HasType U (A::Γ) body B := by
+  have H' := H.strong henv hΓ; clear H hΓ
+  induction H' with
+  | symm _ ih => exact ih eq.symm
+  | trans _ _ ih1 ih2
+  | proofIrrel _ _ _ _ ih1 ih2
+  | extra _ _ _ _ _ _ _ _ _ _ _ _ ih1 ih2 =>
+    obtain eq | eq := eq <;> [exact ih1 (.inl eq); exact ih2 (.inr eq)]
+  | lamDF _ _ h1 _ _ h4 h5 =>
+    obtain ⟨⟨⟩⟩ | ⟨⟨⟩⟩ := eq
+    · exact ⟨⟨_, h1.defeq.hasType.1⟩, _, h4.defeq.hasType.1⟩
+    · exact ⟨⟨_, h1.defeq.hasType.2⟩, _, h5.defeq.hasType.2⟩
+  | defeqDF _ _ _ _ ih2 => exact ih2 eq
+  | beta _ _ _ _ _ _ _ _ _ _ _ _ _ ihee =>
+    obtain ⟨⟨⟩⟩ | eq := eq
+    exact ihee (.inl eq)
+  | eta _ _ hA _ _ _ he' _ _ _ ih =>
+    obtain ⟨⟨⟩⟩ | eq := eq
+    · exact ⟨⟨_, hA.defeq.hasType.1⟩, _, .app he'.defeq.hasType.1 (.bvar .zero)⟩
+    · exact ih (.inl eq)
+  | _ => match eq with.
+
+variable (henv : Ordered env) (hΓ : OnCtx Γ (env.IsType U)) in
+theorem HasType.lam_inv (H : env.HasType U Γ (.lam A body) V) :
+    env.IsType U Γ A ∧ ∃ B, env.HasType U (A::Γ) body B :=
+  H.lam_inv' henv hΓ (.inl rfl)
+
+variable (henv : Ordered env) (hΓ : OnCtx Γ (env.IsType U)) in
+theorem IsDefEq.const_inv'
+    (H : env.IsDefEq U Γ e1 e2 V) (eq : e1 = .const c ls ∨ e2 = .const c ls) :
+    ∃ ci, env.constants c = some (some ci) ∧ (∀ l ∈ ls, l.WF U) ∧ ls.length = ci.uvars := by
+  have H' := H.strong henv hΓ; clear H hΓ
+  induction H' with
+  | symm _ ih => exact ih eq.symm
+  | trans _ _ ih1 ih2
+  | proofIrrel _ _ _ _ ih1 ih2
+  | extra _ _ _ _ _ _ _ _ _ _ _ _ ih1 ih2 =>
+    obtain eq | eq := eq <;> [exact ih1 (.inl eq); exact ih2 (.inr eq)]
+  | constDF h1 h2 h3 h4 h5 _ _ =>
+    obtain ⟨⟨⟩⟩ | ⟨⟨⟩⟩ := eq
+    · exact ⟨_, h1, h2, h4⟩
+    · exact ⟨_, h1, h3, h5.length_eq.symm.trans h4⟩
+  | defeqDF _ _ _ _ ih2 => exact ih2 eq
+  | beta _ _ _ _ _ _ _ _ _ _ _ _ _ ihee =>
+    obtain ⟨⟨⟩⟩ | eq := eq
+    exact ihee (.inl eq)
+  | eta _ _ _ _ _ _ _ _ _ _ ih =>
+    obtain ⟨⟨⟩⟩ | eq := eq
+    exact ih (.inl eq)
+  | _ => match eq with.
+
+variable (henv : Ordered env) (hΓ : OnCtx Γ (env.IsType U)) in
+theorem HasType.const_inv (H : env.HasType U Γ (.const c ls) V) :
+    ∃ ci, env.constants c = some (some ci) ∧ (∀ l ∈ ls, l.WF U) ∧ ls.length = ci.uvars :=
+  H.const_inv' henv hΓ (.inl rfl)
