Lean4Lean/Std/Basic.lean
@@ -17,6 +17,42 @@ protected theorem List.Forall₂.rfl
   | nil => constructor
   | cons _ _ ih => simp at h; exact .cons h.1 (ih h.2)
 
+@[simp] theorem List.forall₂_nil_left_iff {l} : Forall₂ R nil l ↔ l = nil :=
+  ⟨fun H => by cases H; rfl, by rintro rfl; exact Forall₂.nil⟩
+
+@[simp] theorem List.forall₂_nil_right_iff {l} : Forall₂ R l nil ↔ l = nil :=
+  ⟨fun H => by cases H; rfl, by rintro rfl; exact Forall₂.nil⟩
+
+theorem List.forall₂_cons_left_iff {a l u} :
+    Forall₂ R (a :: l) u ↔ ∃ b u', R a b ∧ Forall₂ R l u' ∧ u = b :: u' :=
+  Iff.intro
+    (fun h => match u, h with | b :: u', Forall₂.cons h₁ h₂ => ⟨b, u', h₁, h₂, rfl⟩)
+    (fun h => match u, h with | _, ⟨_, _, h₁, h₂, rfl⟩ => Forall₂.cons h₁ h₂)
+
+theorem List.forall₂_cons_right_iff {b l u} :
+    Forall₂ R u (b :: l) ↔ ∃ a u', R a b ∧ Forall₂ R u' l ∧ u = a :: u' :=
+  Iff.intro
+    (fun h => match u, h with | b :: u', Forall₂.cons h₁ h₂ => ⟨b, u', h₁, h₂, rfl⟩)
+    (fun h => match u, h with | _, ⟨_, _, h₁, h₂, rfl⟩ => Forall₂.cons h₁ h₂)
+
+theorem List.Forall₂.imp (H : ∀ a b, R a b → S a b)
+    {l₁ l₂} (h : Forall₂ R l₁ l₂) : Forall₂ S l₁ l₂ := by
+  induction h <;> constructor <;> [(apply H; assumption); assumption]
+
+@[simp] theorem List.forall₂_map_left_iff {f : γ → α} :
+    ∀ {l u}, Forall₂ R (map f l) u ↔ Forall₂ (fun c b => R (f c) b) l u
+  | [], _ => by simp only [map, forall₂_nil_left_iff]
+  | a :: l, _ => by simp only [map, forall₂_cons_left_iff, forall₂_map_left_iff]
+
+@[simp] theorem List.forall₂_map_right_iff {f : γ → β} :
+    ∀ {l u}, Forall₂ R l (map f u) ↔ Forall₂ (fun a c => R a (f c)) l u
+  | _, [] => by simp only [map, forall₂_nil_right_iff]
+  | _, b :: u => by simp only [map, forall₂_cons_right_iff, forall₂_map_right_iff]
+
+theorem List.Forall₂.length_eq : ∀ {l₁ l₂}, Forall₂ R l₁ l₂ → length l₁ = length l₂
+  | _, _, Forall₂.nil => rfl
+  | _, _, Forall₂.cons _ h₂ => congrArg Nat.succ (Forall₂.length_eq h₂)
+
 theorem List.map_id' {f : α → α} (l : List α) (h : ∀ x ∈ l, f x = x) : map f l = l := by
   induction l <;> simp_all
 
